Split semtyp_lemmas.later_sub_sem from syntyp_lemmas.later_sub_syn

theories/Dot/syntyp_lemmas/later_sub_syn.v
@@ -2,10 +2,11 @@
 
 
 From D Require Import proper.
+From D.Dot Require Import later_sub_sem.
 From D.Dot Require Import unary_lr.
 From D.Dot Require Import typing_aux_defs.
 From D.Dot Require Import type_eq.
-From D.Dot Require Import dsub_lr.
+From D.Dot Require Import dsub_lr. (* XXX *)
 
 Set Suggest Proof Using.
 Set Default Proof Using "Type".
@@ -56,15 +57,8 @@ Section TypeEquiv.
   Qed.
 End TypeEquiv.
 
-(* This is specialized to [anil] because contexts only contain proper types anyway. *)
-Definition s_ty_sub `{HdlangG: !dlangG Σ} (T1 T2 : oltyO Σ) := ∀ ρ v, T1 anil ρ v -∗ T2 anil ρ v.
-Notation "s⊨T T1 <: T2" := (s_ty_sub T1 T2) (at level 74, T1, T2 at next level).
-
 Definition ty_sub `{HdlangG: !dlangG Σ} T1 T2 := s⊨T V⟦ T1 ⟧ <: V⟦ T2 ⟧.
 Notation "⊨T T1 <: T2" := (ty_sub T1 T2) (at level 74, T1, T2 at next level).
-
-Definition s_ctx_sub `{HdlangG: !dlangG Σ} (Γ1 Γ2 : sCtx Σ) : Prop := ∀ ρ, sG⟦ Γ1 ⟧* ρ -∗ sG⟦ Γ2 ⟧* ρ.
-Notation "s⊨G Γ1 <:* Γ2" := (s_ctx_sub Γ1 Γ2) (at level 74, Γ1, Γ2 at next level).
 
 Definition ctx_sub `{HdlangG: !dlangG Σ} Γ1 Γ2 : Prop := s⊨G V⟦ Γ1 ⟧* <:* V⟦ Γ2 ⟧*.
 Notation "⊨G Γ1 <:* Γ2" := (ctx_sub Γ1 Γ2) (at level 74, Γ1, Γ2 at next level).
@@ -73,52 +67,18 @@ Section CtxSub.
   Context `{HdlangG: !dlangG Σ}.
   Implicit Type (T : ty) (Γ : ctx).
 
-  (** * Basic lemmas about [s_ctx_sub]. *)
-  #[global] Instance: RewriteRelation s_ty_sub := {}.
-  #[global] Instance pre_s_ty_sub: PreOrder s_ty_sub.
-  Proof. split; first done. by move => x y z H1 H2 ρ v; rewrite (H1 _ _). Qed.
-
   #[global] Instance: RewriteRelation ty_sub := {}.
   #[global] Instance: PreOrder ty_sub.
   Proof. rewrite /ty_sub; split; first done. by move => x y z H1 H2; etrans. Qed.
-
-  #[global] Instance: RewriteRelation s_ctx_sub := {}.
-  #[global] Instance: PreOrder s_ctx_sub.
-  Proof. split; first done. by move => x y z H1 H2 ρ; rewrite (H1 _). Qed.
 
   #[global] Instance: RewriteRelation ctx_sub := {}.
   #[global] Instance: PreOrder ctx_sub.
   Proof. rewrite /ctx_sub; split; first done. by move => x y z H1 H2; etrans. Qed.
 
-  #[global] Instance: Proper (equiv ==> equiv ==> iff) s_ctx_sub.
-  Proof.
-    rewrite /s_ctx_sub => Γ1 Γ2 HΓ Δ1 Δ2 HΔ.
-    by setoid_rewrite HΔ; setoid_rewrite HΓ.
-  Qed.
-
-  #[global] Instance cons_s_ctx_sub_proper : Proper (s_ty_sub ==> s_ctx_sub ==> s_ctx_sub) cons.
-  Proof. move => T1 T2 HlT Γ1 Γ2 Hl ρ. cbn. by rewrite (HlT _) (Hl _). Qed.
-  (* This is needed when flip ctx_sub arises from other rules. Doh. *)
-  #[global] Instance cons_s_ctx_sub_flip_proper :
-    Proper (flip s_ty_sub ==> flip s_ctx_sub ==> flip s_ctx_sub) cons.
-  Proof. solve_proper. Qed.
-
   #[global] Instance cons_ctx_sub_proper : Proper (ty_sub ==> ctx_sub ==> ctx_sub) cons.
   Proof. rewrite /ty_sub /ctx_sub. solve_proper. Qed.
   #[global] Instance cons_ctx_sub_flip_proper : Proper (flip ty_sub ==> flip ctx_sub ==> flip ctx_sub) cons.
   Proof. solve_proper. Qed.
-
-  (** Typing is contravariant in [Γ].
-  Note these instances are very specialized. *)
-  #[global] Instance setp_proper e : Proper (flip s_ctx_sub ==> (=) ==> (⊢)) (setp e).
-  Proof. rewrite /setp => Γ1 Γ2 Hweak T1 T2 ->. by setoid_rewrite (Hweak _). Qed.
-  #[global] Instance setp_flip_proper e : Proper (s_ctx_sub ==> flip (=) ==> flip (⊢)) (setp e).
-  Proof. apply: flip_proper_3. Qed.
-
-  #[global] Instance sstpd_proper i : Proper (flip s_ctx_sub ==> (=) ==> (=) ==> (⊢)) (sstpd i).
-  Proof. rewrite /sstpd => Γ1 Γ2 Hweak T1 T2 -> U1 U2 ->. by setoid_rewrite (Hweak _). Qed.
-  #[global] Instance sstpi_flip_proper i : Proper (s_ctx_sub ==> flip (=) ==> flip (=) ==> flip (⊢)) (sstpd i).
-  Proof. apply: flip_proper_4. Qed.
 
   #[global] Instance ietp_proper : Proper (flip ctx_sub ==> (=) ==> (=) ==> (⊢)) ietp.
   Proof.
@@ -139,24 +99,11 @@ Section CtxSub.
     Proper (ctx_sub ==> flip (=) ==> flip (=) ==> flip (⊢)) (istpd i).
   Proof. apply: flip_proper_4. Qed.
 
-
-  #[global] Instance oLater_proper : Proper (s_ty_sub ==> s_ty_sub) oLater.
-  Proof. intros x y Hl ??. by rewrite /= (Hl _ _). Qed.
-  #[global] Instance oLater_flip_proper :
-    Proper (flip s_ty_sub ==> flip s_ty_sub) oLater.
-  Proof. apply: flip_proper_2. Qed.
-
   #[global] Instance TLater_proper : Proper (ty_sub ==> ty_sub) TLater.
   Proof. by rewrite /ty_sub => ?? /= ->. Qed.
   #[global] Instance TLater_flip_proper :
     Proper (flip ty_sub ==> flip ty_sub) TLater.
   Proof. apply: flip_proper_2. Qed.
-
-  Lemma senv_TLater_commute (Γ : sCtx Σ) ρ : sG⟦ oLater <$> Γ ⟧* ρ ⊣⊢ ▷ sG⟦ Γ ⟧* ρ.
-  Proof.
-    elim: Γ ρ => [| T Γ IH] ρ; cbn; [|rewrite IH later_and];
-      iSplit; by [iIntros "$" | iIntros "_"].
-  Qed.
 
   Lemma fmap_TLater_oLater Γ : V⟦ TLater <$> Γ ⟧* = oLater <$> V⟦ Γ ⟧*.
   Proof. elim: Γ => [//| T Γ IH]; cbn. by rewrite IH. Qed.
@@ -285,11 +232,10 @@ Section CtxSub.
   Lemma istpd_weaken_ctx_syn Γ1 Γ2 {T1 T2 i} (Hsyn : ⊢G Γ1 <:* Γ2) :
     Γ2 ⊨ T1 <:[i] T2 -∗ Γ1 ⊨ T1 <:[i] T2.
   Proof. by apply istpd_proper; first apply (fundamental_ctx_sub Hsyn). Qed.
+
 End CtxSub.
 
-Typeclasses Opaque s_ty_sub.
 Typeclasses Opaque ty_sub.
-Typeclasses Opaque s_ctx_sub.
 Typeclasses Opaque ctx_sub.
 
 #[global] Hint Resolve ietp_weaken_ctx_syn fundamental_ctx_sub : ctx_sub.
